code proving

coqimp/contextswitch/proof/CtxSwitchProof.v
@@ -1,11 +1,11 @@
-Require Import Coqlib.                   
-Require Import Maps.          
+Require Import Coqlib.                      
+Require Import Maps.           
 Require Import LibTactics.   
         
 Require Import Integers.  
-Open Scope Z_scope.       
+Open Scope Z_scope.        
 Import ListNotations.  
-  
+   
 Set Asymmetric Patterns.  
         
 Require Import state.    
@@ -34,7 +34,37 @@ Open Scope mem_scope.
 
 Definition spec := convert_spec
                      ((Ta0_return, Ta0_return +ᵢ ($ 4),
-                       (os_ta0_return_pre, os_ta0_return_post)) :: nil).
+                       (os_ta0_return_pre, os_ta0_return_post))
+                        :: (Ta0_Window_OK, Ta0_Window_OK +ᵢ ($ 4),
+                            (ta0_window_ok_pre, ta0_window_ok_post))
+                        :: nil).
+
+(*+ Trivial Lemmas +*)
+Lemma len_neq_0_tail :
+  forall {A : Type} (ls : list A),
+    length ls > 0 -> exists a ls', ls = ls' ++ (a :: nil).
+Proof.
+  intros A ls.
+  induction ls; intros.
+  -
+    simpls; tryfalse.
+    omega.
+  -
+    destruct ls.
+    exists a.
+    eexists.
+    instantiate (1 := nil).
+    simpl; eauto.
+    assert (length (a0 :: ls) > 0).
+    simpl; eauto.
+    omega.
+    eapply IHls in H0.
+    simpljoin1.
+    exists x (a :: x0).
+    simpl; eauto.
+    rewrite H0.
+    eauto.
+Qed.
 
 (*+ Lemmas about TimReduce +*)
 Theorem GenRegs_TimeReduce :
@@ -453,12 +483,563 @@ Proof.
     destruct (zeq (Int.unsigned $ 4) (Int.unsigned $ 4095)) eqn:Heqe3; eauto; tryfalse.
 Qed.
 
+Lemma get_range_0_4_stable :
+  forall id,
+    $ 0 <=ᵤᵢ id <=ᵤᵢ $ 7 -> get_range 0 4 id = id.
+Proof.
+  intros.
+  rewrite <- Int.repr_unsigned.
+  unfold get_range.
+  unfold Int.and.
+  unfold Int.shl.
+  unfold Int.sub.
+  simpl.
+  assert (Int.unsigned $ 1 = 1%Z).
+  simpl; eauto.
+  assert (Int.unsigned $ 5 = 5%Z).
+  simpl; eauto.
+  assert (Int.unsigned $ 0 = 0%Z).
+  simpl; eauto.
+  rewrite H0, H1, H2.
+  simpl.
+  assert (Int.unsigned $ 32 = 32%Z).
+  simpl; eauto.
+  rewrite H3.
+  simpl; eauto.
+  assert (Int.unsigned $ 31 = 31%Z).
+  simpl; eauto.
+  do 2 rewrite H4.
+  destruct id.
+  unfold int_leu, Int.eq, Int.ltu in H.
+  rewrite H2 in H.
+  assert (Int.unsigned $ 7 = 7%Z).
+  simpl; eauto.
+  rewrite H5 in H; eauto.
+  simpl Int.unsigned in H.
+  simpl. 
+  destruct (zlt 0 intval); destruct (zeq 0 intval);
+    destruct (zlt intval 7); destruct (zeq intval 7); simpls; tryfalse; try omega.
+  clear H H0 H1 H2 H3 H4 H5.
+  assert (Z.land intval 31 = intval).
+  {
+    unfold Z.land.
+    destruct intval; tryfalse.
+    clear - l l0.
+    repeat (destruct p; simpl; eauto; tryfalse; try omega).
+  } 
+  rewrite H.
+  eauto.
+  clear H H0 H1 H2 H3 H4 H5.
+  rewrite e; simpl; eauto. 
+  rewrite <- e; simpl; eauto. 
+Qed.
+
+Lemma and_zero_not_eq :
+  forall v1 v2,
+    $ 0 <=ᵤᵢ v1 <=ᵤᵢ $ 7 -> $ 0 <=ᵤᵢ v2 <=ᵤᵢ $ 7 ->
+    (($ 1) <<ᵢ v1) &ᵢ (($ 1) <<ᵢ v2) = $ 0 ->
+    v1 <> v2.
+Proof.
+  intros.
+  intro.
+  subst.
+  rewrite Int.and_idem in H1.
+  clear H.
+  unfolds int_leu.
+  unfolds Int.ltu, Int.eq.
+  rewrite <- Int.repr_unsigned with (i := v2) in H1.
+  destruct v2.
+  simpl Int.unsigned in H0. 
+  assert (Int.unsigned $ 0 = 0%Z).
+  simpl; eauto.
+  assert (Int.unsigned $ 7 = 7%Z).
+  simpl; eauto.
+  rewrite H in H0.
+  rewrite H2 in H0.
+  simpl in H1.
+  destruct (zlt 0 intval);
+    destruct (zeq 0 intval);
+    destruct (zlt intval 7); destruct (zeq intval 7); tryfalse; try omega.
+  {
+    clear - l l0 H1.
+    unfolds Int.shl.
+    assert (Int.unsigned $ 1 = 1%Z).
+    simpl; eauto.
+    rewrite H in H1.
+    clear H.
+    destruct intval; simpls; tryfalse; eauto.
+    destruct p; tryfalse;
+    destruct p; tryfalse;
+    destruct p; tryfalse.
+  }
+  {
+    subst.
+    unfolds Int.shl.
+    rewrite H2 in H1.
+    assert (Int.unsigned $ 1 = 1%Z).
+    simpl; eauto.
+    rewrite H3 in H1.
+    simpls.
+    tryfalse.
+  }
+  {
+    subst.
+    unfolds Int.shl.
+    assert (Int.unsigned $ 1 = 1%Z).
+    simpl; eauto.
+    rewrite H3 in H1.
+    rewrite H in H1.
+    simpls.
+    tryfalse.
+  }
+Qed.
+
+Lemma range_0_7_int_unsigned_eq :
+  forall z,
+    (0 < z)%Z ->  (z < 7)%Z ->
+    Int.unsigned $ z = z.
+Proof.
+  intros.
+  rewrite Int.unsigned_repr_eq.
+  unfold Int.modulus.
+  unfold two_power_nat.
+  simpl.
+  destruct z; tryfalse.
+  destruct p; tryfalse; eauto;
+    destruct p; tryfalse; eauto;
+      destruct p; tryfalse; eauto.
+Qed.
+
+Lemma range_0_7_shiftl_int_unsigned_eq :
+  forall z,
+    (0 < z)%Z ->  (z < 7)%Z ->
+    Int.unsigned $ (Z.shiftl 1 z) = Z.shiftl 1 z.
+Proof.
+  intros.
+  rewrite Int.unsigned_repr_eq.
+  unfold Int.modulus.
+  unfold two_power_nat.
+  simpl.
+  destruct z; tryfalse.
+  destruct p; tryfalse; eauto;
+    destruct p; tryfalse; eauto;
+      destruct p; tryfalse; eauto.
+Qed.
+
+Lemma range_0_7_add_7_eq :
+  forall z,
+    (0 < z)%Z ->  (z < 7)%Z ->
+    Int.unsigned $ (z + 7) = (z + 7)%Z.
+Proof.
+  intros.
+  rewrite Int.unsigned_repr_eq.
+  unfold Int.modulus.
+  unfold two_power_nat.
+  simpl.
+  destruct z; tryfalse.
+  destruct p; tryfalse; eauto;
+    destruct p; tryfalse; eauto;
+      destruct p; tryfalse; eauto.
+Qed.
+
+Lemma range_0_7_add_8_eq :
+  forall z,
+    (0 < z)%Z ->  (z < 7)%Z ->
+    Int.unsigned $ (z + 8) = (z + 8)%Z.
+Proof.
+  intros.
+  rewrite Int.unsigned_repr_eq.
+  unfold Int.modulus.
+  unfold two_power_nat.
+  simpl.
+  destruct z; tryfalse.
+  destruct p; tryfalse; eauto;
+    destruct p; tryfalse; eauto;
+      destruct p; tryfalse; eauto.
+Qed.
+
+Lemma and_not_zero_eq :
+  forall v1 v2,
+    $ 0 <=ᵤᵢ v1 <=ᵤᵢ $ 7 -> $ 0 <=ᵤᵢ v2 <=ᵤᵢ $ 7 ->
+    (($ 1) <<ᵢ v1) &ᵢ (($ 1) <<ᵢ v2) <> $ 0 ->
+    v1 = v2.
+Proof.
+  intros.
+  rewrite <- Int.repr_unsigned with (i := v1).
+  rewrite <- Int.repr_unsigned with (i := v2).
+  rewrite <- Int.repr_unsigned with (i := v1) in H1.
+  rewrite <- Int.repr_unsigned with (i := v2) in H1.
+  unfolds int_leu.
+  unfolds Int.ltu.
+  unfolds Int.eq.
+  assert (Int.unsigned $ 0 = 0%Z).
+  simpl; eauto.
+  assert (Int.unsigned $ 7 = 7%Z).
+  simpl; eauto.
+  try rewrite H2 in *.
+  try rewrite H3 in *.
+  destruct v1, v2.
+  simpl Int.unsigned in *.
+  unfolds Int.shl.
+  assert (Int.unsigned $ 1 = 1%Z).
+  simpl; eauto.
+  try rewrite H4 in *.
+  unfold Int.and in H1.
+  destruct (zlt 0 intval);
+    destruct (zeq 0 intval); destruct (zlt intval 7); destruct (zeq intval 7);
+      destruct (zlt 0 intval0);
+      destruct (zeq 0 intval0); destruct (zlt intval0 7); destruct (zeq intval0 7);
+        tryfalse; simpls; subst; eauto; try omega.
+  {
+    rewrite range_0_7_int_unsigned_eq with (z := intval) in H1; eauto.
+    rewrite range_0_7_int_unsigned_eq with (z := intval0) in H1; eauto.
+    rewrite range_0_7_shiftl_int_unsigned_eq in H1; eauto.
+    rewrite range_0_7_shiftl_int_unsigned_eq in H1; eauto.
+    
+    destruct intval, intval0; simpl; eauto; try omega; tryfalse.
+    destruct p; destruct p0;
+      try destruct p; try destruct p0;
+        try destruct p; try destruct p0; tryfalse; simpl; eauto; simpls; tryfalse;
+          try solve [unfolds Int.unsigned; simpls; tryfalse].
+  }
+  {
+    rewrite range_0_7_int_unsigned_eq with (z := intval) in H1; eauto.
+    rewrite range_0_7_shiftl_int_unsigned_eq in H1; eauto.
+    rewrite H3 in H1.
+    simpl in H1.
+    assert (Int.unsigned $ 128 = 128%Z).
+    eauto.
+    rewrite H5 in H1.
+
+    destruct intval; simpl; eauto; try omega; tryfalse.
+    destruct p; try destruct p; try destruct p;
+      tryfalse; simpl; eauto; simpls; tryfalse.
+  }
+  {
+    rewrite range_0_7_int_unsigned_eq with (z := intval) in H1; eauto.
+    rewrite range_0_7_shiftl_int_unsigned_eq in H1; eauto.
+    rewrite H2 in H1.
+    simpl in H1.
+    rewrite H4 in H1.
+
+    destruct intval; simpl; eauto; try omega; tryfalse.
+    destruct p; try destruct p; try destruct p;
+      tryfalse; simpl; eauto; simpls; tryfalse.
+  }
+  { 
+    rewrite range_0_7_int_unsigned_eq with (z := intval0) in H1; eauto.
+    rewrite H3 in H1.
+    simpl in H1.
+    assert (Int.unsigned $ 128 = 128%Z).
+    eauto.
+    rewrite H5 in H1.
+    rewrite range_0_7_shiftl_int_unsigned_eq in H1; eauto.
+
+    destruct intval0; simpl; eauto; try omega; tryfalse.
+    destruct p; try destruct p; try destruct p;
+      tryfalse; simpl; eauto; simpls; tryfalse.
+  }
+  {
+    rewrite H3 in H1.
+    rewrite H2 in H1.
+    simpls.
+    assert (Int.unsigned $ 128 = 128%Z).
+    eauto.
+    rewrite H5 in H1.
+    rewrite H4 in H1.
+    simpls.
+    tryfalse.
+  }
+  {
+    rewrite range_0_7_int_unsigned_eq with (z := intval0) in H1; eauto.
+    rewrite H2 in H1.
+    simpl in H1.
+    rewrite H4 in H1.
+    rewrite range_0_7_shiftl_int_unsigned_eq in H1; eauto.
+
+    destruct intval0; simpl; eauto; try omega; tryfalse.
+    destruct p; try destruct p; try destruct p;
+      tryfalse; simpl; eauto; simpls; tryfalse.
+  }
+  {
+    rewrite H3 in H1.
+    rewrite H2 in H1.
+    simpls.
+    rewrite H4 in H1.
+    assert (Int.unsigned $ 128 = 128%Z).
+    eauto.
+    rewrite H5 in H1.
+    simpls.
+    tryfalse.
+  }
+Qed.
+
+Lemma in_range_0_7_pre_cwp_still :
+  forall id,
+    $ 0 <=ᵤᵢ id <=ᵤᵢ $ 7 ->
+    $ 0 <=ᵤᵢ (pre_cwp id) <=ᵤᵢ $ 7.
+Proof.
+  intros.
+  unfold pre_cwp.
+  unfolds int_leu.
+  unfolds Int.ltu.
+  unfolds Int.eq.
+  unfold N.
+  unfold Int.add.
+  unfold Int.sub.
+  assert (Int.unsigned $ 0 = 0%Z).
+  eauto.
+  assert (Int.unsigned $ 7 = 7%Z).
+  eauto.
+  assert (Int.unsigned $ 8 = 8%Z).
+  eauto.
+  assert (Int.unsigned $ 1 = 1%Z).
+  eauto.
+  try rewrite H0 in *.
+  try rewrite H1 in *.
+  try rewrite H2 in *.
+  try rewrite H3 in *.
+  destruct id.
+  simpl Int.unsigned in *.
+  destruct (zlt 0 intval);
+    destruct (zeq 0 intval); destruct (zlt intval 7); destruct (zeq intval 7);
+      eauto; tryfalse; try omega.
+  {
+    destruct intval; eauto; tryfalse.
+    destruct p;
+      try destruct p; try destruct p; tryfalse; try omega; eauto.
+  }
+  {
+    subst.
+    eauto.
+  }
+  {
+    subst.
+    eauto.
+  }
+Qed.
+
+Lemma in_range_0_7_post_cwp_still :
+  forall id,
+    $ 0 <=ᵤᵢ id <=ᵤᵢ $ 7 ->
+    $ 0 <=ᵤᵢ (post_cwp id) <=ᵤᵢ $ 7.
+Proof.
+  intros.
+  unfold post_cwp.
+  unfolds int_leu.
+  unfolds Int.ltu.
+  unfolds Int.eq.
+  unfold N.
+  unfold Int.add.
+  unfold Int.sub.
+  assert (Int.unsigned $ 0 = 0%Z).
+  eauto.
+  assert (Int.unsigned $ 7 = 7%Z).
+  eauto.
+  assert (Int.unsigned $ 8 = 8%Z).
+  eauto.
+  assert (Int.unsigned $ 1 = 1%Z).
+  eauto.
+  try rewrite H0 in *.
+  try rewrite H1 in *.
+  try rewrite H2 in *.
+  try rewrite H3 in *.
+  destruct id.
+  simpl Int.unsigned in *.
+  destruct (zlt 0 intval);
+    destruct (zeq 0 intval); destruct (zlt intval 7); destruct (zeq intval 7);
+      eauto; tryfalse; try omega.
+  {
+    destruct intval; eauto; tryfalse.
+    destruct p;
+      try destruct p; try destruct p; tryfalse; try omega; eauto.
+  }
+  {
+    subst.
+    eauto.
+  }
+  {
+    subst.
+    eauto.
+  }
+Qed.
+
+Lemma win_mask_pre_cwp :
+  forall id,
+    $ 0 <=ᵤᵢ id <=ᵤᵢ $ 7 ->
+    (($ 1) <<ᵢ (pre_cwp id)) &ᵢ (($ 1) <<ᵢ id) = $ 0.
+Proof.
+  intros.
+  unfolds int_leu.
+  unfolds Int.ltu.
+  unfolds Int.eq.
+  assert (Int.unsigned $ 0 = 0%Z).
+  eauto.
+  assert (Int.unsigned $ 7 = 7%Z).
+  eauto.
+  assert (Int.unsigned $ 1 = 1%Z).
+  eauto.
+  assert (Int.unsigned $ 8 = 8%Z).
+  eauto.
+  unfold pre_cwp.
+  unfold Int.and.
+  unfold Int.shl.
+  unfold Int.add.
+  unfold Int.sub.
+  unfold N.
+  try rewrite H0 in *.
+  try rewrite H1 in *.
+  try rewrite H2 in *.
+  try rewrite H3 in *.
+  destruct id.
+  simpl Int.unsigned in *.
+  destruct (zlt 0 intval); destruct (zeq 0 intval);
+    destruct (zlt intval 7); destruct (zeq intval 7); tryfalse; try omega.
+  {
+    rewrite range_0_7_add_8_eq; eauto.
+    assert ((intval + 8 - 1 = intval + 7)%Z).
+    omega.
+    rewrite H4.
+    unfold Int.modu.
+    rewrite H3.
+    destruct intval; eauto; tryfalse.
+    do 3 (try destruct p; eauto; tryfalse).
+  }
+  {
+    subst.
+    unfold Int.modu.
+    simpl.
+    rewrite H3.
+    eauto.
+  }
+  {
+    subst.
+    unfold Int.modu.
+    rewrite H3.
+    simpl.
+    eauto.
+  }
+Qed.
+  
 Ltac eval_spec :=
   match goal with
   | |- ?spec (?f1, ?f2) = Some (?fp, ?fq) =>
     unfold spec; unfold convert_spec;
     repeat progress (destruct_addreq; destruct_addreq)
   end.
+
+(*+ Lemmas for asrt +*)
+Lemma asrt_disj_intro :
+  forall p1 p2 s,
+    s |= p1 \/ s |= p2 ->
+    s |= p1 \\// p2.
+Proof.
+  intros.
+  simpl.
+  eauto.
+Qed.
+
+(*+ Lemmas for Rules +*)
+Lemma rd_rule_reg_wim :
+  forall (v id : Word) (rr : GenReg) (p : asrt) F (grst : GenRegState),
+    |- {{GenRegs grst ** FrameState id v F ** p}} rd Rwim rr
+      {{GenRegs (upd_genreg grst rr (($ 1) <<ᵢ v)) ** FrameState id v F ** p}}.
+Proof.
+  intros.
+  eapply ins_conseq_rule.
+  introv Hs. 
+  simpl_sep_liftn_in Hs 2.
+  unfold FrameState in Hs.
+  eapply astar_assoc_elim in Hs.
+  simpl_sep_liftn_in Hs 2.
+  eapply astar_assoc_elim in Hs.
+  simpl_sep_liftn_in Hs 4.
+  eauto.
+  eapply rd_rule_reg.
+  introv Hs.
+  sep_cancel1 1 1.
+  unfold FrameState.
+  eapply astar_assoc_intro.
+  sep_cancel1 3 1.
+  eapply astar_assoc_intro.
+  sep_cancel1 1 1.
+  eauto.
+Qed.
+
+Theorem save_rule_reg_frame :
+  forall p (rs rd : GenReg) (id id' : Word) (F : FrameList)
+    (fm1 fm2 fmg fmo fml fmi : Frame) (v1 v2 v v' : Word) (oexp : OpExp),
+    get_genreg_val (fmg, fmo, fml, fmi) rs = v1 ->
+    eval_opexp_reg (fmg, fmo, fml, fmi) oexp = Some v2 ->
+    id' = pre_cwp id -> win_masked id' (($ 1) <<ᵢ v) = false ->
+    |- {{ GenRegs (fmg, fmo, fml, fmi) ** FrameState id v (F ++ fm1 :: fm2 :: nil) ** p }}
+        save rs oexp rd
+        {{ GenRegs (upd_genreg (fmg, fm1, fm2, fmo) rd (v1 +ᵢ v2)) **
+                   FrameState id' v (fml :: fmi :: F) ** p }}.
+Proof.
+  intros.
+  eapply ins_conseq_rule.
+  Focus 2.
+  eapply save_rule_reg; eauto.
+  {
+    introv Hs.
+    instantiate (4 := F).
+    instantiate (3 := fm1).
+    instantiate (2 := fm2).
+    instantiate (1 := [|length (fml :: fmi :: F) = 13|]
+                        ** [|$ 0 <=ᵤᵢ id' <=ᵤᵢ $ 7 /\ $ 0 <=ᵤᵢ v <=ᵤᵢ $ 7|] ** p).
+    unfolds FrameState.
+    sep_cancel1 1 1.
+    eapply astar_assoc_elim in H3.
+    sep_cancel1 1 2.
+    eapply astar_assoc_elim in H4.
+    sep_cancel1 1 1.
+    eapply astar_assoc_elim in H3.
+    eapply sep_pure_l_elim in H3.
+    simpljoin1.
+    eapply sep_pure_l_elim in H4.
+    simpljoin1; eauto.
+    eapply sep_pure_l_intro.
+    rewrite app_length in H3.
+    simpls.
+    omega. 
+    eapply sep_pure_l_intro; eauto.
+    split; eauto.
+    eapply in_range_0_7_pre_cwp_still; eauto.
+  }
+  {
+    introv Hs.
+    sep_cancel1 1 1.
+    unfold FrameState.
+    eapply astar_assoc_intro.
+    sep_cancel1 2 1.
+    eapply astar_assoc_intro.
+    sep_cancel1 1 1.
+    eapply astar_assoc_intro; eauto.
+  }
+Qed.
+
+(*+ Lemmas for stack frame constraint +*)
+Lemma stack_frame_constraint_pt_same_equal :
+  forall fm1 fm2 fm1' fm2' F id vi stk,
+    get_frame_nth fm2 6 = get_frame_nth fm2' 6 ->
+    stack_frame_constraint stk (fm1 :: fm2 :: F) id vi ->
+    stack_frame_constraint stk (fm1' :: fm2' :: F) id vi.
+Proof.
+  intros.
+  unfolds stack_frame_constraint.
+  inversion H0; subst.
+  {
+    eapply frame_invalid; eauto.
+  }
+  {
+    eapply frame_valid; eauto.
+    inversion H2; subst.
+    rewrite <- H; eauto.
+    inversion H2; subst.
+    eauto.
+  }
+Qed.
   
 (*+ Proof +*)
 Theorem OSInt0HandlerProof :
@@ -693,5 +1274,229 @@ Proof.
   TimReduce_simpl.
   eapply set_rule_reg; eauto.
   simpl upd_genreg.
+
+  (** sll l5 l4 l5 *)
+  eapply seq_rule.
+  TimReduce_simpl.
+  eapply sll_rule_reg; eauto.
+  simpl upd_genreg.
+ 
+  eapply hoare_pure_gen' with ($ 0 <=ᵤᵢ id <=ᵤᵢ $ 7 /\ $ 0 <=ᵤᵢ vi <=ᵤᵢ $ 7).
+  introv Hs.
+  simpl_sep_liftn_in Hs 6.
+  unfold FrameState in Hs.
+  do 3 (eapply astar_assoc_elim in Hs; simpl_sep_liftn_in Hs 2).
+  eapply sep_pure_l_elim in Hs; simpljoin1; eauto.
   
+  eapply Pure_intro_rule.
+  introv Hid_range.
+  destruct Hid_range as [Hid_range Hvi_range].
+  lets Hget_rang_id : Hid_range.
+  eapply get_range_0_4_stable in Hget_rang_id.
+  rewrite Hget_rang_id.
+ 
+  (** rd wim l4 *)
+  hoare_lift_pre 6.
+  hoare_lift_pre 2.
+  eapply seq_rule.
+  TimReduce_simpl.
+  eapply rd_rule_reg_wim; eauto.
+  simpl upd_genreg.
+
+  (** andcc l4 l5 g0 *) 
+  hoare_lift_pre 5.
+  hoare_lift_pre 5.
+  hoare_lift_pre 3.
+  eapply seq_rule.
+  TimReduce_simpl.
+  eapply andcc_rule_reg; eauto.
+  simpl; eauto.
+  simpl upd_genreg.
+  simpl get_genreg_val.
+
+  unfold iszero at 1.
+  destruct (Int.eq_dec (($ 1) <<ᵢ vi) &ᵢ (($ 1) <<ᵢ id) $ 0).
+  {
+    (** be Ta0_Window_OK; nop *)
+    eapply Be_rule.
+    {
+      eval_spec.
+    }
+    {
+      TimReduce_simpl.
+      eapply nop_rule; eauto.
+    }
+    {
+      introv Hs.
+      TimReduce_simpl_in Hs.
+      sep_cancel1 3 1.
+      simpl; eauto.
+    }
+    {
+      introv Hcontr.
+      eapply int_eq_true_eq in Hcontr; tryfalse.
+    }
+
+    instantiate (1 := Aemp).
+    simpl; eauto.
+    introv Hneq.
+    split.
+    { 
+      introv Hs.
+      unfold ta0_window_ok_pre.
+      sep_ex_intro.
+      asrt_to_line 30.
+      eapply sep_pure_l_intro; eauto.
+      simpl_sep_liftn 2.
+      eapply GenRegs_split_Regs_Global.
+      sep_cancel1 1 1.
+      sep_cancel1 3 1.
+      sep_cancel1 1 3.
+      sep_cancel1 1 2.
+      sep_cancel1 2 4.
+      sep_cancel1 2 1.
+      sep_cancel1 2 1.
+      sep_cancel1 2 1.
+      sep_cancel1 2 1.
+      sep_cancel1 2 1.
+      sep_cancel1 2 1.
+      match goal with
+      | H : _ |= _ |- _ => renames H to Hs
+      end.
+      asrt_to_line_in Hs 20.
+      sep_cancel1 1 3.
+      sep_cancel1 1 3.
+      eapply sep_pure_l_intro.
+      simpl; eauto.
+      eapply and_zero_not_eq in e; eauto.
+      eapply sep_pure_l_intro; eauto.
+      sep_cancel1 1 1.
+      sep_cancel1 1 1.
+      match goal with
+      | H : _ |= _ |- _ => renames H to Hs
+      end.
+      eapply sep_pure_l_elim in Hs.
+      destruct Hs as [Hstk_frame_constraint Hs].
+      eapply sep_pure_l_intro; eauto.
+      introv Hcctx_offset.
+      eapply Hstk_frame_constraint in Hcctx_offset.
+      eapply stack_frame_constraint_pt_same_equal; eauto.
+    }
+    { 
+      unfold ta0_window_ok_post.
+      introv Hs.
+      sep_ex_elim_in Hs.
+      asrt_to_line_in Hs 100.
+      eapply sep_pure_l_elim in Hs.
+      destruct Hs as [Hlv Hs]. 
+      inversion Hlv; subst.
+      clear Hlv.
+      sep_ex_intro.
+      eapply sep_pure_l_intro; eauto.
+      do 14 sep_cancel1 1 1.
+      eapply asrt_disj_intro.
+      right.
+      eapply sep_pure_l_intro; eauto.
+      sep_cancel1 1 1.
+      sep_cancel1 1 1.
+      sep_cancel1 2 2.
+      simpl update_frame.
+      match goal with
+      | H : _ |= _ |- _ => renames H to Hs
+      end. 
+      eapply sep_pure_l_elim in Hs.
+      destruct Hs as [Hctx_save Hs].
+      eapply sep_pure_l_intro; eauto.
+    }
+  }
+ 
+  rename n into Hwin_invalid.
+  eapply and_not_zero_eq in Hwin_invalid; eauto.
+  subst vi.
+
+  (** be Ta0_Window_OK; nop *)
+  eapply Be_rule.
+  {
+    eval_spec.
+  }
+  {
+    TimReduce_simpl.
+    eapply nop_rule; eauto.
+  }
+ 
+  introv Hs.
+  TimReduce_simpl_in Hs.
+  sep_cancel1 3 1.
+  simpl; eauto.
+
+  Focus 2.
+  instantiate (1 := Aemp).
+  simpl; eauto.
+
+  Focus 2.
+  introv Hcontr.
+  eapply int_eq_false_neq in Hcontr.
+  tryfalse.
+
+  introv Heq.
+  clear Heq.
+  rewrite Int.and_idem.
+
+  eapply hoare_pure_gen' with (pu := length F = 13).
+  {
+    introv Hs.
+    simpl_sep_liftn_in Hs 4.
+    unfold FrameState in Hs.
+    eapply astar_assoc_elim in Hs.
+    simpl_sep_liftn_in Hs 2.
+    eapply astar_assoc_elim in Hs.
+    simpl_sep_liftn_in Hs 2.
+    eapply astar_assoc_elim in Hs.
+    eapply sep_pure_l_elim in Hs.
+    simpljoin1; eauto.
+  }
+
+  eapply Pure_intro_rule.
+  introv Hlen_F.
+  assert (HF_tail : length F > 0).
+  omega.
+  eapply len_neq_0_tail in HF_tail.
+  destruct HF_tail as [fm [F' HF_tail ] ].
+  subst F.
+  destruct fm.
+  rewrite <- app_assoc.
+  simpl app.
+  destruct cstk as [l lfp].
+  rewrite app_length in Hlen_F.
+  simpl in Hlen_F.
+  assert (Hlen_F' : length F' = 12).
+  omega.
+  clear Hlen_F.
+  assert (HF_tail : length F' > 0).
+  omega.
+  eapply len_neq_0_tail in HF_tail.
+  destruct HF_tail as [fm [F'' HF_tail ] ].
+  destruct fm.
+  subst F'.
+  do 2 rewrite <- app_assoc.
+  simpl app.
+  hoare_lift_pre 4.
+  hoare_lift_pre 2.
+
+  (** save *)
+  eapply seq_rule.
+  TimReduce_simpl.
+  eapply save_rule_reg_frame; eauto.
+  simpl. eauto.
+  unfold win_masked.
+  destruct (((($ 1) <<ᵢ (pre_cwp id)) &ᵢ (($ 1) <<ᵢ id)) !=ᵢ ($ 0)) eqn:Heqe; eauto.
+  unfold negb in Heqe.
+  destruct (((($ 1) <<ᵢ (pre_cwp id)) &ᵢ (($ 1) <<ᵢ id)) =ᵢ ($ 0)) eqn:Heqe1; tryfalse.
+  eapply int_eq_false_neq in Heqe1.
+  false.
+  eapply Heqe1.
+  clear - Hid_range.
+  eapply win_mask_pre_cwp; eauto.
+  simpl upd_genreg.
+    
   >>>>>>>>>>>>>>>
